First try on proving correctness for the if statement.

LambdaS5/coq/LjsAuxiliary.v
@@ -4,14 +4,3 @@ Require Import LjsShared.
 Require Import Utils.
 Require Import LjsSyntax.
 
-Definition object_binds st ptr obj :=
-    Heap.binds (object_heap st) ptr obj.
-
-Definition object_indom st ptr :=
-    Heap.indom (object_heap st) ptr.
-
-Definition id_binds c i loc :=
-    Heap.binds (value_heap c) i loc.
-
-Definition id_indom c i :=
-    Heap.indom (value_heap c) i.
