LambdaS5/coq/LjsPrettyRulesAux.v
@@ -1,0 +1,52 @@
+Generalizable All Variables.
+Set Implicit Arguments.
+Require Import Utils.
+Require Import LjsShared.
+Require Import LjsSyntax.
+Require Import LjsPrettyInterm.
+Require Import LjsPrettyRules.
+Require Import LjsStore.
+Require Import LjsCommon.
+Require Import LjsValues.
+Require Import LjsOperators.
+Require Import LjsMonads.
+Require Import JsNumber.
+Require Import Coq.Strings.String.
+Import List.ListNotations.
+
+Open Scope list_scope.
+
+Implicit Type st : store.
+Implicit Type e : expr.
+Implicit Type v : value.
+Implicit Type s : string.
+Implicit Type n : number.
+Implicit Type i : id.
+Implicit Type o : out.
+Implicit Type c : ctx.
+Implicit Type ptr : object_ptr.
+Implicit Type obj : object.
+
+Lemma out_red_ter : forall c st st' ee r o,
+    red_expr c st ee (out_ter st' r) -> out_of_ext_expr ee = Some o -> exists st'' r', o = out_ter st'' r'.
+Proof.
+    introv Hred Hout.
+    unfolds in Hout;
+    inverts Hred; tryfalse; injects; jauto.
+Qed.
+ 
+Module Export Tactics.
+
+Ltac ljs_out_red_ter Hred :=
+    let H := fresh in
+    forwards (?st&?r&H) : out_red_ter Hred; [reflexivity | ]; 
+    match type of H with ?x = _ => is_var x end; 
+    rewrite H in *; clear H.
+
+Tactic Notation "ljs_out_red_ter" "in" hyp(Hred) := ljs_out_red_ter Hred.
+
+Tactic Notation "ljs_out_red_ter" := match goal with 
+    | H : red_expr _ _ _ (out_ter _ _) |- _ => ljs_out_red_ter in H
+    end.
+
+End Tactics.
